verification/proofs/Chunk_hexVal/obl_0_60_2.lean
@@ -3,4 +3,4 @@
   subst hrun
   simp only [State.set, Nat.reduceEqDiff, reduceIte]
   rw [wrap_id' (by omega) (by omega)]
-  rw [hexValF_of (by unfold digitVal; rw [ if_pos (And.intro (by omega) (by omega))])]
+  rw [hexValF_of (by unfold digitVal; rw [if_neg (by omega), if_neg (by omega),  if_pos (And.intro (by omega) (by omega))])]
