verification/proofs/Chunk_hexVal/obl_0_64_0.lean
@@ -1,4 +1,4 @@
-  simp only [inv_22, inv_46, inv_70, inv_79]
+  simp only [inv_22, inv_41, inv_60, inv_64]
   simp [run, step, P, hpc, hstk, State.set, pLt, pGt, *] at hrun
   subst hrun
   simp only [State.set, Nat.reduceEqDiff, reduceIte]
